update based on POPL AE feedback

theories/F_mu_ref/binary/examples/fact.v
@@ -5,22 +5,22 @@ From WBLogic.F_mu_ref.binary Require Import soundness rules.
 From iris.prelude Require Import options.
 
 Definition fact : expr :=
-  Rec (If (BinOp Eq (Var 1) (#n 0))
-          (#n 1)
-          (BinOp Mult (Var 1) (App (Var 0) (BinOp Sub (Var 1) (#n 1))))).
+  Rec (If (BinOp Eq (Var 1) (#z 0))
+          (#z 1)
+          (BinOp Mult (Var 1) (App (Var 0) (BinOp Sub (Var 1) (#z 1))))).
 
 Definition factV : val :=
-  RecV (If (BinOp Eq (Var 1) (#n 0))
-          (#n 1)
-          (BinOp Mult (Var 1) (App (Var 0) (BinOp Sub (Var 1) (#n 1))))).
+  RecV (If (BinOp Eq (Var 1) (#z 0))
+          (#z 1)
+          (BinOp Mult (Var 1) (App (Var 0) (BinOp Sub (Var 1) (#z 1))))).
 
-Lemma fact_typed : [] ⊢ₜ fact : TArrow TNat TNat.
+Lemma fact_typed : [] ⊢ₜ fact : TArrow TInt TInt.
 Proof. repeat econstructor. Qed.
 
 Lemma fact_unfold :
-  fact = Rec (If (BinOp Eq (Var 1) (#n 0))
-                 (#n 1)
-                 (BinOp Mult (Var 1) (App (Var 0) (BinOp Sub (Var 1) (#n 1))))).
+  fact = Rec (If (BinOp Eq (Var 1) (#z 0))
+                 (#z 1)
+                 (BinOp Mult (Var 1) (App (Var 0) (BinOp Sub (Var 1) (#z 1))))).
 Proof. done. Qed.
 
 Global Typeclasses Opaque fact.
@@ -31,19 +31,19 @@ Global Opaque factV.
 
 Definition fact_acc_body : expr :=
   Rec (Lam
-         (If (BinOp Eq (Var 2) (#n 0))
+         (If (BinOp Eq (Var 2) (#z 0))
              (Var 0)
              (LetIn
                 (BinOp Mult (Var 2) (Var 0))
                 (LetIn
-                   (BinOp Sub (Var 3) (#n 1))
+                   (BinOp Sub (Var 3) (#z 1))
                    (App (App (Var 3) (Var 0)) (Var 1))
                 )
              )
          )
       ).
 
-Lemma fact_acc_body_typed : [] ⊢ₜ fact_acc_body : TArrow TNat (TArrow TNat TNat).
+Lemma fact_acc_body_typed : [] ⊢ₜ fact_acc_body : TArrow TInt (TArrow TInt TInt).
 Proof. repeat econstructor. Qed.
 
 Lemma fact_acc_body_subst f : fact_acc_body.[f] = fact_acc_body.
@@ -54,12 +54,12 @@ Global Hint Rewrite fact_acc_body_subst : autosubst.
 Lemma fact_acc_body_unfold :
   fact_acc_body =
   Rec (Lam
-         (If (BinOp Eq (Var 2) (#n 0))
+         (If (BinOp Eq (Var 2) (#z 0))
              (Var 0)
              (LetIn
                 (BinOp Mult (Var 2) (Var 0))
                 (LetIn
-                   (BinOp Sub (Var 3) (#n 1))
+                   (BinOp Sub (Var 3) (#z 1))
                    (App (App (Var 3) (Var 0)) (Var 1))
                 )
              )
@@ -71,18 +71,18 @@ Global Typeclasses Opaque fact_acc_body.
 Global Opaque fact_acc_body.
 
 Definition fact_acc : expr :=
-  Lam (App (App fact_acc_body (Var 0)) (#n 1)).
+  Lam (App (App fact_acc_body (Var 0)) (#z 1)).
 
 Definition fact_accV : val :=
-  LamV (App (App fact_acc_body (Var 0)) (#n 1)).
+  LamV (App (App fact_acc_body (Var 0)) (#z 1)).
 
-Lemma fact_acc_unfold : fact_acc = Lam (App (App fact_acc_body (Var 0)) (#n 1)).
+Lemma fact_acc_unfold : fact_acc = Lam (App (App fact_acc_body (Var 0)) (#z 1)).
 Proof. done. Qed.
 
 Lemma fact_acc_subst f : fact_acc.[f] = fact_acc.
 Proof. by asimpl. Qed.
 
-Lemma fact_acc_typed : [] ⊢ₜ fact_acc : TArrow TNat TNat.
+Lemma fact_acc_typed : [] ⊢ₜ fact_acc : TArrow TInt TInt.
 Proof.
   repeat econstructor.
   apply (closed_context_weakening [_] []); eauto.
@@ -99,7 +99,7 @@ Section fact_equiv.
   Context `{heapIG Σ, cfgSG Σ, ghost_regG Σ}.
 
   Lemma fact_fact_acc_refinement :
-    ⊢ [] ⊨ fact ≤log≤ fact_acc : (TArrow TNat TNat).
+    ⊢ [] ⊨ fact ≤log≤ fact_acc : (TArrow TInt TInt).
   Proof.
     iIntros (? vs) "!# [#HE HΔ]".
     iDestruct (interp_env_length with "HΔ") as %?; destruct vs; simplify_eq.
@@ -114,78 +114,63 @@ Section fact_equiv.
     iIntros (j K) "Hj"; simpl.
     iMod (do_step_pure with "[$Hj]") as "Hj"; auto.
     asimpl.
-    iApply (wbwp_mono _ _ _ (λ v, ∃ m, j ⤇ fill K (#n (1 * m)) ∗ ⌜v = #nv m⌝))%I.
+    iApply (wbwp_mono _ _ _ (λ v, ∃ m, j ⤇ fill K (#z (1 * m)) ∗ ⌜v = #zv m⌝))%I.
     { iIntros (?). iDestruct 1 as (m) "[? %]"; subst.
-      iExists (#nv _); iFrame; eauto. }
-    generalize 1 as l => l.
-    iInduction n as [|n] "IH" forall (l).
-    - rewrite fact_unfold.
-      iApply wbwp_pure_step_later; auto.
-      rewrite -fact_unfold.
-      iNext; iIntros "_"; simpl; asimpl.
-      rewrite fact_acc_body_unfold.
-      iMod (do_step_pure _ _ (AppLCtx _ :: _) with "[$Hj]") as "Hj"; auto.
-      rewrite -fact_acc_body_unfold.
-      simpl; asimpl.
-      iMod (do_step_pure with "[$Hj]") as "Hj"; auto.
-      iApply (wbwp_bind (fill [IfCtx _ _])).
-      iApply wbwp_pure_step_later; auto.
-      iNext; iIntros "_"; simpl.
-      iApply wbwp_value. simpl.
-      iMod (do_step_pure _ _ (IfCtx _ _ :: _) with "[$Hj]") as "Hj"; auto.
-      simpl.
-      iApply wbwp_pure_step_later; auto.
+      iExists (#zv _); iFrame; iExists _; iSplit; first done.
+      replace (1 * m)%Z with m by lia; done. }
+    generalize 1%Z as l => l.
+    iLöb as "IH" forall (n l).
+    rewrite fact_unfold.
+    iApply wbwp_pure_step_later; auto.
+    rewrite -fact_unfold.
+    iNext; iIntros "_"; simpl; asimpl.
+    rewrite fact_acc_body_unfold.
+    iMod (do_step_pure _ _ (AppLCtx _ :: _) with "[$Hj]") as "Hj"; auto.
+    rewrite -fact_acc_body_unfold.
+    simpl; asimpl.
+    iMod (do_step_pure with "[$Hj]") as "Hj"; auto.
+    iApply (wbwp_bind (fill [IfCtx _ _])).
+    iApply wbwp_pure_step_later; auto.
+    iNext; iIntros "_"; simpl.
+    iApply wbwp_value. simpl.
+    iMod (do_step_pure _ _ (IfCtx _ _ :: _) with "[$Hj]") as "Hj"; auto.
+    destruct Z.eq_dec as [->|].
+    - iApply wbwp_pure_step_later; auto.
       iNext; iIntros "_"; simpl.
       iMod (do_step_pure with "[$Hj]") as "Hj"; auto.
       iApply wbwp_value.
-      iExists 1. replace (l * 1) with l by lia.
-      iFrame; done.
+      iExists _; iFrame; iSplit; last done. replace (l * 1)%Z with l by lia; done.
     - rewrite fact_unfold.
       iApply wbwp_pure_step_later; auto.
       rewrite -fact_unfold.
       iNext; iIntros "_"; simpl; asimpl.
       rewrite fact_acc_body_unfold.
-      iMod (do_step_pure _ _ (AppLCtx _ :: _) with "[$Hj]") as "Hj"; auto.
+      destruct Z.eq_dec; first done.
+      iMod (do_step_pure with "[$Hj]") as "Hj"; auto.
+      iMod (do_step_pure _ _ (LetInCtx _ :: _) with "[$Hj]") as "Hj"; auto.
+      simpl.
+      iMod (do_step_pure with "[$Hj]") as "Hj"; auto.
+      iMod (do_step_pure _ _ (LetInCtx _ :: _) with "[$Hj]") as "Hj"; auto.
+      simpl.
+      iMod (do_step_pure with "[$Hj]") as "Hj"; auto.
       rewrite -fact_acc_body_unfold.
       simpl; asimpl.
-      iMod (do_step_pure with "[$Hj]") as "Hj"; auto.
-      iApply (wbwp_bind (fill [IfCtx _ _])).
-      iApply wbwp_pure_step_later; auto.
-      iNext; iIntros "_"; simpl.
-      iApply wbwp_value. simpl.
-      iMod (do_step_pure _ _ (IfCtx _ _ :: _) with "[$Hj]") as "Hj"; auto.
-      simpl.
-      iApply wbwp_pure_step_later; auto.
-      iNext; iIntros "_"; simpl.
-      iMod (do_step_pure with "[$Hj]") as "Hj"; auto.
-      iAsimpl.
-      iApply (wbwp_bind (fill [BinOpRCtx _ (#nv _)])).
+      iApply (wbwp_bind (fill [BinOpRCtx _ (#zv _)])).
       change fact with (of_val factV).
       iApply (wbwp_bind (fill [AppRCtx _])).
       iApply wbwp_pure_step_later; auto.
       iNext; iIntros "_"; simpl; iApply wbwp_value; simpl.
-      iMod (do_step_pure _ _ (LetInCtx _ :: _) with "[$Hj]") as "Hj"; auto.
-      simpl.
-      change (of_val factV) with fact.
-      iMod (do_step_pure with "[$Hj]") as "Hj"; auto.
-      iAsimpl.
-      iMod (do_step_pure _ _ (LetInCtx _ :: _) with "[$Hj]") as "Hj"; auto.
-      simpl.
-      iMod (do_step_pure with "[$Hj]") as "Hj"; auto.
-      asimpl.
-      replace (n -0) with n by lia.
       iApply wbwp_wand_r; iSplitL; first by iApply ("IH" with "[$]"); eauto.
       iIntros (v). iDestruct 1 as (m) "[H %]"; simplify_eq.
       iApply wbwp_pure_step_later; auto.
       iNext; iIntros "_"; simpl; iApply wbwp_value.
-      iExists ((S n) * m); simpl.
-      replace (l * (m + n * m)) with ((l + n * l) * m)
-        by lia.
+      iExists (n * m)%Z; simpl.
+      replace (l * (n * m))%Z with (n * l * m)%Z by lia.
       iFrame; auto.
   Qed.
 
   Lemma fact_acc_fact_refinement :
-    ⊢ [] ⊨ fact_acc ≤log≤ fact : (TArrow TNat TNat).
+    ⊢ [] ⊨ fact_acc ≤log≤ fact : (TArrow TInt TInt).
   Proof.
     iIntros (? vs) "!# [#HE HΔ]".
     iDestruct (interp_env_length with "HΔ") as %?; destruct vs; simplify_eq.
@@ -200,59 +185,45 @@ Section fact_equiv.
     iIntros (j K) "Hj"; simpl.
     iApply wbwp_pure_step_later; auto.
     iNext; iIntros "_"; iAsimpl.
-    iApply (wbwp_mono _ _ _ (λ v, ∃ m, j ⤇ fill K (#n m) ∗ ⌜v = #nv (1 * m)⌝))%I.
+    iApply (wbwp_mono _ _ _ (λ v, ∃ m, j ⤇ fill K (#z m) ∗ ⌜v = #zv (1 * m)⌝))%I.
     { iIntros (?). iDestruct 1 as (m) "[? %]"; simplify_eq.
-      replace (1 * m) with m by lia.
-      iExists (#nv _); iFrame; eauto. }
-    generalize 1 as l => l.
-    iInduction n as [|n] "IH" forall (K l).
-    - rewrite fact_acc_body_unfold.
-      iApply (wbwp_bind (fill [AppLCtx _])).
-      iApply wbwp_pure_step_later; auto.
-      rewrite -fact_acc_body_unfold.
-      iNext; iIntros "_"; simpl; asimpl.
-      iApply wbwp_value; simpl.
-      iApply wbwp_pure_step_later; auto.
-      iNext; iIntros "_"; simpl; asimpl.
-      rewrite fact_unfold.
-      iMod (do_step_pure with "[$Hj]") as "Hj"; auto.
-      simpl; iAsimpl.
-      rewrite -fact_unfold.
-      iMod (do_step_pure _ _ (IfCtx _ _ :: _) with "[$Hj]") as "Hj"; auto.
-      iApply (wbwp_bind (fill [IfCtx _ _])).
-      iApply wbwp_pure_step_later; auto.
-      iNext; iIntros "_"; simpl.
-      iApply wbwp_value. simpl.
+      replace (1 * m)%Z with m by lia.
+      iExists (#zv _); iFrame; eauto. }
+    generalize 1%Z as l => l.
+    iLöb as "IH" forall (K n l).
+    rewrite fact_acc_body_unfold.
+    iApply (wbwp_bind (fill [AppLCtx _])).
+    iApply wbwp_pure_step_later; auto.
+    rewrite -fact_acc_body_unfold.
+    iNext; iIntros "_"; simpl; asimpl.
+    iApply wbwp_value; simpl.
+    iApply wbwp_pure_step_later; auto.
+    iNext; iIntros "_"; simpl; asimpl.
+    rewrite fact_unfold.
+    iMod (do_step_pure with "[$Hj]") as "Hj"; auto.
+    simpl; iAsimpl.
+    rewrite -fact_unfold.
+    iMod (do_step_pure _ _ (IfCtx _ _ :: _) with "[$Hj]") as "Hj"; auto.
+    iApply (wbwp_bind (fill [IfCtx _ _])).
+    iApply wbwp_pure_step_later; auto.
+    iNext; iIntros "_"; simpl.
+    destruct Z.eq_dec as [->|].
+    - iApply wbwp_value. simpl.
       iMod (do_step_pure with "[$Hj]") as "Hj"; auto.
       iApply wbwp_pure_step_later; auto.
       iNext; iIntros "_"; simpl.
       iApply wbwp_value.
-      iExists 1.
-      replace (l * 1) with l by lia; iFrame; auto.
+      iExists 1%Z.
+      replace (l * 1)%Z with l by lia; iFrame; auto.
     - rewrite {2}fact_acc_body_unfold.
-      iApply (wbwp_bind (fill [AppLCtx _])).
-      iApply wbwp_pure_step_later; auto.
-      rewrite -fact_acc_body_unfold.
-      iNext; iIntros "_"; simpl; asimpl.
       iApply wbwp_value; simpl.
       iApply wbwp_pure_step_later; auto.
       iNext; iIntros "_"; simpl; asimpl.
       rewrite fact_unfold.
       iMod (do_step_pure with "[$Hj]") as "Hj"; auto.
       rewrite -fact_unfold.
-      asimpl.
-      simpl.
-      iApply (wbwp_bind (fill [IfCtx _ _])).
-      iApply wbwp_pure_step_later; auto.
-      iNext; iIntros "_"; simpl.
-      iApply wbwp_value. simpl.
-      iMod (do_step_pure _ _ (IfCtx _ _ :: _) with "[$Hj]") as "Hj"; auto.
-      simpl.
-      iApply wbwp_pure_step_later; auto.
-      iNext; iIntros "_"; simpl.
-      iMod (do_step_pure with "[$Hj]") as "Hj"; auto.
       change fact with (of_val factV).
-      iMod (do_step_pure _ _ (AppRCtx _:: BinOpRCtx _ (#nv _) :: _)
+      iMod (do_step_pure _ _ (AppRCtx _:: BinOpRCtx _ (#zv _) :: _)
              with "[$Hj]") as "Hj"; eauto.
       simpl.
       change (of_val factV) with fact.
@@ -266,25 +237,25 @@ Section fact_equiv.
       iNext; iIntros "_"; simpl; iApply wbwp_value; simpl.
       iApply wbwp_pure_step_later; auto.
       iNext; iIntros "_"; simpl. asimpl.
-      replace (n -0) with n by lia.
+      rewrite -fact_acc_body_unfold.
       iApply wbwp_fupd.
       iApply wbwp_wand_r; iSplitL;
-        first by iApply ("IH" $! (BinOpRCtx _ (#nv _) :: K) with "[$]"); eauto.
+        first by iApply ("IH" $! (BinOpRCtx _ (#zv _) :: K) with "[$]"); eauto.
       iIntros (v). iDestruct 1 as (m) "[Hj %]"; simplify_eq.
       simpl.
       iMod (do_step_pure with "[$Hj]") as "Hj"; auto.
       simpl.
       iModIntro.
-      iExists (S n * m).
+      iExists (n * m)%Z.
       iFrame.
-      eauto with lia.
+      replace (l * (n * m))%Z with (n * l * m)%Z by lia; done.
   Qed.
 
 End fact_equiv.
 
 Theorem fact_ctx_equiv :
-  [] ⊨ fact ≤ctx≤ fact_acc : (TArrow TNat TNat) ∧
-  [] ⊨ fact_acc ≤ctx≤ fact : (TArrow TNat TNat).
+  [] ⊨ fact ≤ctx≤ fact_acc : (TArrow TInt TInt) ∧
+  [] ⊨ fact_acc ≤ctx≤ fact : (TArrow TInt TInt).
 Proof.
   set (Σ := #[invΣ ; gen_heapΣ loc val; soundness_binaryΣ; gstacksΣ]).
   set (HG := soundness.soundness_unary_preIG Σ _ _ _).
