theories/heap_lang_examples/awkward.v
@@ -16,72 +16,68 @@ Definition awkward_self_apply : expr :=
   "f" (λ: <>, "f" (λ: <>, #());; #()).
 
 Section awkward.
-  Context `{!wbheapGS Σ} `{!oneshotG Σ}.
+  Context `{!heapGS Σ} `{!oneshotG Σ}.
 
-  Lemma wbwp_awkward :
-    ⊢ {WB{{ True }}}
+  Lemma wp_awkward :
+    ⊢ {{{ True }}}
       awkward
       {{{(f : val), RET f;
           ∀ (g : val),
-            {WB{{ {WB{{ True }}} g #() {{{ RET #(); True }}} }}} f g {{{ RET #1; True }}}
+            {{{ {{{ True }}} g #() {{{ RET #(); True }}} }}} f g {{{ RET #1; True }}}
       }}}.
   Proof.
     rewrite /awkward.
     iIntros (Φ) "_ !# HΦ".
-    wbwp_alloc l as "Hl".
-    wbwp_pures.
+    wp_alloc l as "Hl".
+    wp_pures.
     iMod new_pending as (γ) "Hpen".
     iMod (inv_alloc
             (nroot .@ "awk") _
             ((pending γ ∗ l ↦ #0) ∨ (shot γ ∗ l ↦ #1))%I with "[Hpen Hl]") as "#Hinv".
     { iNext; iLeft; iFrame. }
-    iApply wbwp_value.
-    iApply "HΦ".
+    iModIntro; iApply "HΦ".
     clear Φ.
     iIntros (g) "!#".
     iIntros (Φ) "#Hg HΦ".
-    wbwp_pures.
-    wbwp_bind (_ <- _)%E.
+    wp_pures.
+    wp_bind (_ <- _)%E.
     iInv (nroot .@ "awk") as ">Hl" "Hcl".
     iAssert (∃ v, l ↦ v ∗ (pending γ ∨ shot γ))%I with "[Hl]" as (?) "[Hl Hps]".
     { iDestruct "Hl" as "[[? ?]|[? ?]]"; iExists _; iFrame. }
     iAssert (|==> shot γ)%I with "[Hps]" as ">#Hsh".
     { iDestruct "Hps" as "[Hp|Hs]"; last done. iApply shoot; done. }
-    wbwp_store.
-    iApply wbwp_value.
+    wp_store.
     iMod ("Hcl" with "[Hl]") as "_".
     { iNext; iRight; iFrame; done. }
     iModIntro.
-    wbwp_pures.
-    wbwp_apply "Hg"; first done.
+    wp_pures.
+    wp_apply "Hg"; first done.
     iIntros "_".
-    wbwp_pures.
+    wp_pures.
     iInv (nroot .@ "awk") as ">Hl" "Hcl".
     iDestruct "Hl" as "[[Hp _]|[_ Hl]]".
     { iExFalso; iApply shot_not_pending; done. }
-    wbwp_load.
-    iApply wbwp_value.
+    wp_load.
     iMod ("Hcl" with "[Hl]") as "_".
     { iNext; iRight; iFrame; done. }
     iModIntro.
     iFrame. iApply "HΦ"; done.
   Qed.
 
-  Lemma wbwp_awkward_self_apply :
-    ⊢ WBWP awkward_self_apply {{v, ⌜v = #1⌝}}.
+  Lemma wp_awkward_self_apply :
+    ⊢ WP awkward_self_apply {{v, ⌜v = #1⌝}}.
   Proof.
     rewrite /awkward_self_apply.
-    wbwp_apply wbwp_awkward; first done.
+    wp_apply wp_awkward; first done.
     iIntros (f) "#Hf".
-    wbwp_pures.
-    wbwp_apply "Hf"; last done.
+    wp_pures.
+    wp_apply "Hf"; last done.
     iIntros "!#" (Φ) "_ HΦ".
-    wbwp_pures.
-    wbwp_apply "Hf"; last first.
-    { iIntros; wbwp_pures; iApply wbwp_value; iApply "HΦ"; done. }
+    wp_pures.
+    wp_apply "Hf"; last first.
+    { iIntros; wp_pures; iApply "HΦ"; done. }
     iIntros "!#" (Ψ) "_ HΨ".
-    wbwp_pures.
-    iApply wbwp_value.
+    wp_pures.
     iApply "HΨ"; done.
   Qed.
 
@@ -91,6 +87,6 @@ Theorem awkward_self_apply_returns_one σ :
   adequate NotStuck awkward_self_apply σ (λ v _, v = #1).
 Proof.
   set (Σ := #[heapΣ; oneshotΣ]).
-  apply (wbheap_adequacy Σ).
-  iIntros (?) "?". iApply wbwp_awkward_self_apply.
+  apply (heap_adequacy Σ).
+  iIntros (?) "?". iApply wp_awkward_self_apply.
 Qed.
